\chapter{Classical Goppa Codes}
Next we introduce classical Goppa codes. The original proposal of McElice used these codes in its construction. In addition they remain as one of the few codes proposed for with no publicly known structural attacks, atleast if they are chosen correctly.

\begin{theorem}\label{thm:inverse}
  Let $f \in \mathbb{F}_q[X]$ and $\alpha \in \mathbb{F}_q$ such that $f(\alpha) \neq 0$, then the inverse of $(X - \alpha_i)$ exists in the quotient ring $\frac{\mathbb{F}_{q}[X]}{\gen{f}}$, and may be computed as $-\left(\frac{f(X) - f(\alpha_{i})}{X - \alpha_{i}}\right)f(\alpha_{i})^{-1}$.
\end{theorem}

\begin{proof}
  Follows from the fact that:
  \begin{align*}
-\left(\frac{f(X) - f(\alpha_{i})}{X - \alpha_{i}}\right)f(\alpha_{i})^{-1}(X - \alpha_i) &= - f(\alpha_{i})^{-1} (f(X) - f(\alpha_{i})) \\ &= -f(\alpha_{i})^{-1} f(X) + 1 \equiv 1 \mod f
  \end{align*}
  Which is equivalent with $-\left(\frac{f(X) - f(\alpha_{i})}{X - \alpha_{i}}\right)f(\alpha_{i})^{-1}(X - \alpha_i) = 1 \in \frac{\mathbb{F}_{q}[X]}{\gen{f}}$.
\end{proof}

\begin{definition}\label{def:classical}
  Let $x \in \mathbb{F}_q^n$ and $f \in \mathbb{F}_q[X]$ such that $f(x_i) \neq 0$ for $i = 1, 2, \ldots, n$ and $\mathbb{F}_{q_0} \subseteq \mathbb{F}_q$ be a subfield, then the \textit{classical Goppa code} associated with $(x, f, \mathbb{F}_{q_0})$ is defined as:
  \begin{align*}
    \Gamma(x, f, \mathbb{F}_{q_0}) :&= \left\{c \in \mathbb{F}^n_{q_0} \middle| \sum^n_{i = 1} \frac{c_{i}}{X - x_{i}} \equiv 0 \mod f\right\}
     \\&= \left\{c \in \mathbb{F}^n_{q_0} \middle| \sum^n_{i = 1} \frac{c_{i}}{X - x_{i}} = 0 \in \frac{\mathbb{F}_q[X]}{\gen{f}}\right\}
  \end{align*}
  If $f$ is irreducible, then $\Gamma(x, f, \mathbb{F}_{q_0})$ is also called irreducible.
\end{definition}
From Theorem \ref{thm:inverse} and Definition \ref{def:classical} it follows that $c = (c_1, c_2, \ldots, c_{n}) \in \Gamma(x, f, \mathbb{F}_{q_0})$ if and only if
\begin{equation}\label{eq:condtion_on_coef}
  -\sum_{i = 1}^n c_i \frac{1}{f(x_i)} \frac{f(X) - f(x_i)}{X - x_i} = 0 \in \frac{\mathbb{F}_{q}[X]}{\gen{f}}
\end{equation}
additionally if $f = \sum_{j = 0}^{\deg(f)} a_j X^j$, then:
\begin{align*}
  -\frac{1}{f(x_i)}\frac{f(X) - f(x_i)}{X - x_{i}} &= -\frac{1}{f(x_{i})} \frac{\sum_{j=0}^{\deg(f)} a_{j}(X^j - x_i^j)}{X - x_i} \\ &\stackrel{(a)}= -\frac{1}{f(x_i)} \sum^{\deg(f)}_{j = 1} a_j \sum^{j - 1}_{k = 0} X^k x_i^{j - 1 - k}\\
  &\stackrel{(b)}= -\frac{1}{f(x_{i})} \sum^{\deg(f) - 1}_{k = 0} X^k \left(\sum^{\deg(f)}_{j = k + 1} a_j x_i^{j - 1 - k}\right)
\end{align*}
where $(a)$ follows by polynomial division and $(b)$ from interchanging the sums. Thus:
\begin{equation}\label{eq:yields_pcm}
  \sum_{i = 1}^n \frac{c_i}{X - x_i} = -\sum^n_{i = 1} \frac{c_{i}}{f(x_{i})} \sum_{k = 0}^{\deg(f) - 1} X^k \sum_{j = k + 1}^{\deg(f)} a_j x_i^{j - 1 - k}
\end{equation}
Equation \eqref{eq:yields_pcm} must equal $0$ since $c \in \Gamma(x, f, \mathbb{F}_{q_0})$ which is the case if and only if the coefficients of each $X^k$ is zero, which yields the following proposition:
\begin{proposition}\label{prop:pcm_classical_goppa}
  Let $x \in \mathbb{F}_q^n$ and $f \in \mathbb{F}_q[X]$ with $l := \deg(f)$, then the classical gopppa code $\Gamma(x, f, \mathbb{F}_{q_0})$ has parity check matrix:
  \begin{equation*}
    H = \begin{bmatrix}
          f(x_{1})^{-1} a_{l} & f(x_{2})^{-1} a_{l} & \cdots & f(x_{n})^{-1} a_{l} \\
          f(x_{1})^{-1} (a_{l} + a_{l - 1}x_1) & f(x_{2})^{-1} (a_{l} + a_{l - 1}x_2) & \cdots & f(x_{n})^{-1} (a_{l} + a_{l - 1}x_n) \\
          \vdots & \vdots & \ddots & \vdots \\
          f(x_{1})^{-1} \sum_{j = 1}^l a_j x_1^{j -  1} & f(x_{2})^{-1} \sum_{j = 1}^l a_j x_2^{j -  1} & \cdots & f(x_{n})^{-1} \sum_{j = 1}^l a_j x_n^{j -  1} &
        \end{bmatrix}
  \end{equation*}
  over $\mathbb{F}_q$.
\end{proposition}
The following Corollary uses some elementary results from \textcolor{blue}{Galois} theory, namely that if $\mathbb{F}_{q_0}$ is a subfield of the finite field $\mathbb{F}_q$, then there exists a $\mathbb{F}_{q_0}$-basis of $\mathbb{F}_q$. We will denote the length of such a basis by $[\mathbb{F}_q : \mathbb{F}_{q_0}]$ an call it the \textit{degree} of the field extension $\mathbb{F}_q / \mathbb{F}_{q_0}$. \textcolor{blue}{Could be proven in an appendix.}
\begin{corollary}
  Let $\Gamma(x, f, \mathbb{F}_{q_0})$ be a classical goppa code with $x \in \mathbb{F}_q$ and $f \in \mathbb{F}_q[X]$ then:
  \begin{equation*}
    \dim_{\mathbb{F}_{q_0}}(\Gamma(x, f, \mathbb{F}_{q_0})) \geq n - m \deg(f)
  \end{equation*}
  where $m = [\mathbb{F}_q : \mathbb{F}_{q_0}]$.
\end{corollary}
\begin{proof}
  Fixing a $\mathbb{F}_{q_0}$-basis of $\mathbb{F}_q$ say $b_1, b_2, \ldots, b_{m} \in \mathbb{F}_q$, each entry in $H$ can be viewed as a vector in $\mathbb{F}_{q_0}^m$, by the vector space isomorphism:
  \begin{equation*}
  \mathbb{F}_q \ni x =  x_1 b_1 + x_2 b_2 + \cdots + x_m b_m \mapsto \begin{bmatrix} x_1 & x_2 & \cdots & x_{m} \end{bmatrix}^{T} \in \mathbb{F}_{q_0}^m
  \end{equation*}
  Thus $H$ from Proposition \ref{prop:pcm_classical_goppa} can be viewed as a $\mathbb{F}_{q_0}$-matrix $H'$ with dimensions $m \deg(f) \times n$. Since $H'$ has $mt$ rows, we see that $\rank(H') \leq m \deg(f)$, hence
  \begin{equation*}
    \dim_{\mathbb{F}_{q_0}}(\Gamma(x, f, \mathbb{F}_{q_0})) = \dim_{\mathbb{F}_{q_0}}(\Null(H')) = n - \rank(H') \geq n - m \deg(f) \qedhere
  \end{equation*}
\end{proof}

Finally we reach the main theorem of this chapter.

\begin{theorem}\label{thm:classical_goppa_is_AG}
  Let $\Gamma(x, f, \mathbb{F}_q)$ be a classical Goppa code, $P_i = (x_i : 1)$ for $i = 1, 2, \ldots, n$ and $D = \sum_{i = 1}^n P_i$. Then:
  \begin{equation}\label{eq:goppa_is_eval}
    \Gamma(x, f, \mathbb{F}_q) = \mathcal{C}_{\Omega}(\mathbb{P}^1, D, (f)_{0} - P_{\infty}) = \mathcal{C}_L(\mathbb{P}^1, D, (\omega) + D - (f_0) + P_{\infty})
  \end{equation}
  with $\omega = \frac{dh}{h}$ where $h(x) := \prod^n_{i = 1} (x - x_{i})$.
\end{theorem}
\begin{proof}
  The last equality in Equation \eqref{eq:goppa_is_eval} follows by Theorem \ref{thm:res_is_eval}. Hence it is sufficient to show the first equality. We start by showing that $\Gamma(x, f, \mathbb{F}_q) \subseteq \mathcal{C}_{\Omega}(\mathbb{P}^1, D, (f)_0 - P_{\infty})$. Hence let $c \in \Gamma(x, f, \mathbb{F}_q)$ and
  \begin{equation*}
    \omega_c := \left(\sum_{i=1}^n \frac{c_{i}}{x - x_{i}} \right) dx
  \end{equation*}
  by the definition of $\Gamma(x, f, \mathbb{F}_q)$ we see that $v_{P}(\omega_c) \geq 0$ for all $P \in \support((f)_{0})$. In addition $v_{P_i}(\omega_c) = -1$ and $\omega_c$ is regular at any other point $\mathbb{P}^1 \setminus \left\{P_\infty\right\}$. Finally we compute $v_{P_\infty}(\omega_c)$ by setting $x = 1/u$, we see that:
  \begin{equation*}
    \omega_c = \sum_{i=1}^n  \frac{-c_{i} \frac{du}{u^{2}}}{\frac{1}{u} - x_i} = - \sum^n_{i = 1} \frac{c_{i} du}{u(1 - x_{i}u)}
  \end{equation*}
  thus $v_{P_\infty}(\omega_{c}) \geq -1$ and hence $\omega_c \in \Omega((f)_0 - P_{\infty} - D)$ meaning $\Gamma(x, f, \mathbb{F}_q) \subseteq \mathcal{C}_{\Omega}(\mathbb{P}^1, D, (f)_0 - P_{\infty})$.
  \textcolor{red}{\textbf{TODO}} Conversely
\end{proof}
Since Theorem \ref{thm:classical_goppa_is_AG} shows that classical Goppa codes are in fact AG codes it makes sense to speak about their designed minimum distance. This leads us to the following corollary:
\begin{corollary}\label{cor:f_splitting_yields_design_distance}
  If $f \in \mathbb{F}_q[X]$ splits into linear factors over $\mathbb{F}_q$, then:
\begin{equation*}
  d^{*}\left(\Gamma(f, x, \mathbb{F}_q)\right) = \deg(f) + 1
\end{equation*}
\end{corollary}
\begin{proof}
  Using Theorem \ref{thm:classical_goppa_is_AG} we see that:
  \begin{align*}
    d^{*}(\Gamma(f, x, \mathbb{F}_q)) &=d^{*}(\mathcal{C}_L(\mathbb{P}^1, D, (\omega) + D - (f)_0 + P_{\infty}))\\
                                      &= n - \deg((\omega) + D - (f)_0 + P_{\infty}) \\
                                      &\stackrel{(a)}= n - \left(\deg((\omega)) + \deg(D) - \deg((f)_{0}) + \deg(P_{\infty})\right) \\
    &\stackrel{(b)}= n - \left(- 2 + n - \deg(f) + 1\right) \\
    &= \deg(f) + 1
  \end{align*}
  Where $(a)$ follows since $\deg\colon Div(\mathbb{P}^1) \to \mathbb{N}$ is a homomorphism, and Equality $(b)$, follows by $\deg((f)_0) = \deg(f)$ since $f$ factors into linear polynomials and $\deg((\omega)) = -2$ by Proposition \ref{prop:degree_of_canonical_divisor}, with $g = 0$ since $\mathcal{X} = \mathbb{P}^{1}$.
\end{proof}


\input{main/classical_goppa/subfield_subcodes}
